linking: port to dual nondeterminism

theories/interop/linking.v
@@ -91,71 +91,85 @@ Section Linking.
 
   Local Notation prog := (gmap string func).
 
-  Definition proj1_prog (P : prog) : mlanguage.prog Λ1 :=
-    omap (λ fn, match fn with inl fn1 => Some fn1 | inr _ => None end) P.
-  Definition proj2_prog (P : prog) : mlanguage.prog Λ2 :=
-    omap (λ fn, match fn with inl _ => None | inr fn2 => Some fn2 end) P.
+  Definition proj1_prog (p : prog) : mlanguage.prog Λ1 :=
+    omap (λ fn, match fn with inl fn1 => Some fn1 | inr _ => None end) p.
+  Definition proj2_prog (p : prog) : mlanguage.prog Λ2 :=
+    omap (λ fn, match fn with inl _ => None | inr fn2 => Some fn2 end) p.
 
-  Inductive head_step (P : prog) : expr → state → expr → state → Prop :=
+  Implicit Types X : expr * state → Prop.
+
+  Inductive head_step_mrel (p : prog) : expr * state → (expr * state → Prop) → Prop :=
   (* Internal step of an underlying module. *)
-  | Step1S e1 e1' σ1 σ1' privσ2 :
-    prim_step (proj1_prog P) e1 σ1 e1' σ1' →
-    head_step P (LkSE (LinkExpr1 e1)) (LinkSt1 σ1 privσ2) (LkSE (LinkExpr1 e1')) (LinkSt1 σ1' privσ2)
-  | Step2S e2 e2' σ2 σ2' privσ1 :
-    prim_step (proj2_prog P) e2 σ2 e2' σ2' →
-    head_step P (LkSE (LinkExpr2 e2)) (LinkSt2 privσ1 σ2) (LkSE (LinkExpr2 e2')) (LinkSt2 privσ1 σ2')
+  | Step1S e1 σ1 privσ2 (X1 : _ → Prop) X :
+    prim_step (proj1_prog p) (e1, σ1) X1 →
+    (∀ e1' σ1', X1 (e1', σ1') → X (LkSE (LinkExpr1 e1'), LinkSt1 σ1' privσ2)) →
+    head_step_mrel p (LkSE (LinkExpr1 e1), LinkSt1 σ1 privσ2) X
+  | Step2S e2 σ2 privσ1 (X2 : _ → Prop) X :
+    prim_step (proj2_prog p) (e2, σ2) X2 →
+    (∀ e2' σ2', X2 (e2', σ2') → X (LkSE (LinkExpr2 e2'), LinkSt2 privσ1 σ2')) →
+    head_step_mrel p (LkSE (LinkExpr2 e2), LinkSt2 privσ1 σ2) X
   (* Entering a function. Change the view of the heap in the process. *)
-  | RunFunction1S σ1 pubσ privσ1 privσ2 fn1 args e1 :
+  | RunFunction1S σ1 pubσ privσ1 privσ2 fn1 args e1 X :
     mlanguage.apply_func fn1 args = Some e1 →
     mlanguage.split_state σ1 pubσ privσ1 →
-    head_step P (LkSE (LinkRunFunction (inl fn1) args)) (LinkSt pubσ privσ1 privσ2)
-                (LkSE (LinkExpr1 e1)) (LinkSt1 σ1 privσ2)
-  | RunFunction2S σ2 pubσ privσ1 privσ2 fn2 arg e2 :
+    X (LkSE (LinkExpr1 e1), LinkSt1 σ1 privσ2) →
+    head_step_mrel p (LkSE (LinkRunFunction (inl fn1) args), LinkSt pubσ privσ1 privσ2) X
+  | RunFunction2S σ2 pubσ privσ1 privσ2 fn2 arg e2 X :
     mlanguage.apply_func fn2 arg = Some e2 →
     mlanguage.split_state σ2 pubσ privσ2 →
-    head_step P (LkSE (LinkRunFunction (inr fn2) arg)) (LinkSt pubσ privσ1 privσ2)
-                (LkSE (LinkExpr2 e2)) (LinkSt2 privσ1 σ2)
+    X (LkSE (LinkExpr2 e2), LinkSt2 privσ1 σ2) →
+    head_step_mrel p (LkSE (LinkRunFunction (inr fn2) arg), LinkSt pubσ privσ1 privσ2) X
   (* Producing a value when execution is finished *)
-  | Val1S e1 v σ1 pubσ privσ1 privσ2 :
+  | Val1S e1 v σ1 pubσ privσ1 privσ2 X :
     to_val e1 = Some v →
     mlanguage.split_state σ1 pubσ privσ1 →
-    head_step P (LkSE (LinkExpr1 e1)) (LinkSt1 σ1 privσ2)
-                (LkSE (LinkExprV v)) (LinkSt pubσ privσ1 privσ2)
-  | Val2S e2 v σ2 pubσ privσ1 privσ2 :
+    X (LkSE (LinkExprV v), LinkSt pubσ privσ1 privσ2) →
+    head_step_mrel p (LkSE (LinkExpr1 e1), LinkSt1 σ1 privσ2) X
+  | Val2S e2 v σ2 pubσ privσ1 privσ2 X :
     to_val e2 = Some v →
     mlanguage.split_state σ2 pubσ privσ2 →
-    head_step P (LkSE (LinkExpr2 e2)) (LinkSt2 privσ1 σ2)
-                (LkSE (LinkExprV v)) (LinkSt pubσ privσ1 privσ2)
+    X (LkSE (LinkExprV v), LinkSt pubσ privσ1 privσ2) →
+    head_step_mrel p (LkSE (LinkExpr2 e2), LinkSt2 privσ1 σ2) X
   (* Continuing execution by returning a value to its caller *)
-  | Ret1S v k1 σ1 pubσ privσ1 privσ2 :
+  | Ret1S v k1 σ1 pubσ privσ1 privσ2 X :
     mlanguage.split_state σ1 pubσ privσ1 →
-    head_step P (LkE (LinkExprV v) [inl k1]) (LinkSt pubσ privσ1 privσ2)
-                (LkSE (LinkExpr1 (mlanguage.fill k1 (of_val Λ1 v)))) (LinkSt1 σ1 privσ2)
-  | Ret2S v k2 σ2 pubσ privσ1 privσ2 :
+    X (LkSE (LinkExpr1 (mlanguage.fill k1 (of_val Λ1 v))), LinkSt1 σ1 privσ2) →
+    head_step_mrel p (LkE (LinkExprV v) [inl k1], LinkSt pubσ privσ1 privσ2) X
+  | Ret2S v k2 σ2 pubσ privσ1 privσ2 X :
     mlanguage.split_state σ2 pubσ privσ2 →
-    head_step P (LkE (LinkExprV v) [inr k2]) (LinkSt pubσ privσ1 privσ2)
-                (LkSE (LinkExpr2 (mlanguage.fill k2 (of_val Λ2 v)))) (LinkSt2 privσ1 σ2)
+    X (LkSE (LinkExpr2 (mlanguage.fill k2 (of_val Λ2 v))), LinkSt2 privσ1 σ2) →
+    head_step_mrel p (LkE (LinkExprV v) [inr k2], LinkSt pubσ privσ1 privσ2) X
   (* Stuck module calls bubble up as calls at the level of the linking module.
      (They may get unstuck then, if they match a function implemented by the
      other module.) *)
-  | MakeCall1S k1 e1 fn_name arg σ1 pubσ privσ1 privσ2 :
+  | MakeCall1S k1 e1 fn_name arg σ1 pubσ privσ1 privσ2 X :
     mlanguage.to_class e1 = Some (ExprCall fn_name arg) →
-    proj1_prog P !! fn_name = None →
+    proj1_prog p !! fn_name = None →
     mlanguage.split_state σ1 pubσ privσ1 →
-    head_step P (LkSE (LinkExpr1 (mlanguage.fill k1 e1))) (LinkSt1 σ1 privσ2)
-                (LkE (LinkExprCall fn_name arg) [inl k1]) (LinkSt pubσ privσ1 privσ2)
-  | MakeCall2S k2 e2 fn_name arg σ2 pubσ privσ1 privσ2 :
+    X (LkE (LinkExprCall fn_name arg) [inl k1], LinkSt pubσ privσ1 privσ2) →
+    head_step_mrel p (LkSE (LinkExpr1 (mlanguage.fill k1 e1)), LinkSt1 σ1 privσ2) X
+  | MakeCall2S k2 e2 fn_name arg σ2 pubσ privσ1 privσ2 X :
     mlanguage.to_class e2 = Some (ExprCall fn_name arg) →
-    proj2_prog P !! fn_name = None →
+    proj2_prog p !! fn_name = None →
     mlanguage.split_state σ2 pubσ privσ2 →
-    head_step P (LkSE (LinkExpr2 (mlanguage.fill k2 e2))) (LinkSt2 privσ1 σ2)
-                (LkE (LinkExprCall fn_name arg) [inr k2]) (LinkSt pubσ privσ1 privσ2)
+    X (LkE (LinkExprCall fn_name arg) [inr k2], LinkSt pubσ privσ1 privσ2) →
+    head_step_mrel p (LkSE (LinkExpr2 (mlanguage.fill k2 e2)), LinkSt2 privσ1 σ2) X
   (* Resolve an internal call to a module function *)
-  | CallS fn_name fn arg σ :
-    P !! fn_name = Some fn →
-    head_step P (LkSE (LinkExprCall fn_name arg)) σ
-                (LkSE (LinkRunFunction fn arg)) σ.
+  | CallS fn_name fn arg σ X :
+    p !! fn_name = Some fn →
+    X (LkSE (LinkRunFunction fn arg), σ) →
+    head_step_mrel p (LkSE (LinkExprCall fn_name arg), σ) X.
 
+  Program Definition head_step (p : prog) : umrel (expr * state) :=
+    {| mrel := head_step_mrel p |}.
+  Next Obligation.
+    intros p. intros [[se k] σ] X Y Hstep HXY. inversion Hstep; subst;
+      [ eapply Step1S | eapply Step2S | eapply RunFunction1S | eapply RunFunction2S
+      | eapply Val1S | eapply Val2S | eapply Ret1S | eapply Ret2S
+      | eapply MakeCall1S | eapply MakeCall2S | eapply CallS ]; eauto.
+  Qed.
+
+  #[local] Hint Constructors matching_expr_state : core.
   Lemma mlanguage_mixin :
     MlanguageMixin (val:=val) of_class to_class empty_ectx comp_ectx fill
       split_state matching_expr_state apply_func head_step.
@@ -164,11 +178,11 @@ Section Linking.
     - intros c. destruct c; reflexivity.
     - intros e c. destruct e as [e k]. destruct e; cbn.
       1,2: destruct k. all: inversion 1; cbn; auto.
-    - intros p v σ e σ'. cbn. inversion 1.
-    - intros p fn_name v σ e σ'. split.
+    - intros p v σ X. cbn. inversion 1.
+    - intros p fn_name v σ X. split.
       + cbn. inversion 1; subst; naive_solver.
-      + intros [fn (? & Hfn & ->)]. cbn.
-        unfold apply_func in Hfn; simplify_eq; by constructor.
+      + intros (fn & e2 & (? & Hfn & HX)). cbn.
+        unfold apply_func in Hfn; simplify_eq. econstructor; eauto.
     - intros ? ? [? ?] ? ?. rewrite /fill /=. intros. simplify_eq/=; eauto.
     - intros [e k]. rewrite /fill /empty_ectx app_nil_r //.
     - intros K1 K2 [e k]. rewrite /fill /comp_ectx app_assoc //.
@@ -179,11 +193,16 @@ Section Linking.
       assert (k ++ K ≠ []). { intros [? ?]%app_eq_nil. done. }
       cbn in Hsome. destruct (k ++ K) eqn:?.
       2: destruct e; by inversion Hsome. by destruct e.
-    - intros p e1 σ1 e2 σ2 Hmatch. inversion 1; simplify_eq/=; try by constructor.
-      1,2: by (constructor; inversion Hmatch; subst; eauto using matching_expr_state_prim_step).
-      1,2: by (constructor; eauto using apply_func_split_matching).
-      1,2: by (constructor; apply matching_expr_state_ctx; eauto using val_split_matching).
-      inversion Hmatch; subst. constructor.
+    - intros p e1 σ1 X Hmatch. inversion 1; simplify_eq.
+      1,2: econstructor; [eapply matching_expr_state_prim_step; eauto|];
+             inversion Hmatch; naive_solver.
+      1,2: econstructor; naive_solver (eauto using apply_func_split_matching).
+      1,2: econstructor; naive_solver (eauto using matching_expr_state_ctx,val_split_matching).
+      1,2: econstructor; try split; eauto; constructor; apply matching_expr_state_ctx;
+        by eauto using val_split_matching.
+      by eapply MakeCall1S; eauto.
+      by eapply MakeCall2S; eauto.
+      eapply CallS; eauto; inversion Hmatch; naive_solver.
     - intros K e σ. split.
       + inversion 1; subst; simpl; constructor; eauto.
       + destruct e as [? ?]; simpl. inversion 1; subst; constructor; eauto.
@@ -191,12 +210,12 @@ Section Linking.
     - intros *. simpl. inversion 1; subst. do 2 eexists. econstructor.
     - intros *. inversion 1; subst. constructor.
     - intros *. simpl. inversion 1; subst. do 2 eexists. econstructor.
-    - intros p K' K_redex [e1' k1'] [e1_redex k1_redex] σ1 [e2 k2] σ2.
+    - intros p K' K_redex [e1' k1'] [e1_redex k1_redex] σ X.
       rewrite /fill. inversion 1; subst.
       destruct e1_redex; destruct k1' as [|u1' k1']; cbn; try by inversion 1.
       all: intros _; inversion 1; subst; unfold comp_ectx; cbn; eauto.
       all: naive_solver.
-    - intros p K [e k] σ1 [e2 k2] σ2. rewrite /fill. inversion 1; subst.
+    - intros p K [e k] σ X. rewrite /fill. inversion 1; subst.
       all: try match goal with H : _ |- _ => symmetry in H; apply app_nil in H end.
       all: try match goal with H : _ |- _ => symmetry in H; apply app_singleton in H end.
       all: naive_solver.
